Validator/Expr/IfExpr.lean
@@ -7,7 +7,7 @@ import Validator.Expr.Grammar
 inductive IfExpr n α where
   | mk (cnd: Pred α) (thn: Fin n)
 
-abbrev IfExprs n α l := List.Vector (IfExpr n α) l
+abbrev IfExprs n α l := Vec (IfExpr n α) l
 
 namespace IfExpr
 
@@ -19,9 +19,9 @@ def eval {α: Type} [DecidableEq α] (g: Grammar n (Pred α)) (ifExpr: IfExpr n 
     else Regex.emptyset
 
 def evals {α: Type} {n: Nat} [DecidableEq α] (g: Grammar n (Pred α)) (ifExprs: IfExprs n α l) (t: α): Rules n (Pred α) l :=
-  List.Vector.map (fun x => eval g x t) ifExprs
+  Vec.map ifExprs (fun x => eval g x t)
 
 theorem evals_nil_is_nil {α: Type} {n: Nat} [DecidableEq α] (g: Grammar n (Pred α)) (a: α):
-  evals g (n := n) List.Vector.nil a = List.Vector.nil := by
+  evals g (n := n) Vec.nil a = Vec.nil := by
   unfold evals
-  simp
+  simp only [Vec.map_nil]
