Validator/Derive/Leave.lean
@@ -1,3 +1,5 @@
+import Validator.Std.Vec
+
 import Validator.Expr.Grammar
 import Validator.Expr.Regex
 import Validator.Expr.Symbol
@@ -10,15 +12,15 @@ namespace Leave
 -- Each bool will then replace each symbol expression with either an emptystr or emptyset.
 def deriveLeaves
   (xs: Rules n (Pred α) l)
-  (ns: List.Vector Bool (Symbol.nums xs))
+  (ns: Vec Bool (Symbol.nums xs))
   : (Rules n (Pred α) l) :=
   let (regexes, symbols) := Symbol.extractsFrom xs
-  let res: List.Vector ((Pred α × Ref n) × Bool) (Symbol.nums xs) := Vec.zip symbols ns
-  let res': List.Vector (Regex ((Pred α × Ref n) × Bool)) l := Symbol.replacesFrom regexes res
+  let res: Vec ((Pred α × Ref n) × Bool) (Symbol.nums xs) := Vec.zip symbols ns
+  let res': Vec (Regex ((Pred α × Ref n) × Bool)) l := Symbol.replacesFrom regexes res
   Regex.smartDerives2 res'
 
-def deriveLeaveM [Monad m] {n: Nat} {l: Nat} (xs: Rules n (Pred α) l) (ns: List.Vector Bool (Symbol.nums xs)): m (Rules n (Pred α) l) := do
+def deriveLeaveM [Monad m] {n: Nat} {l: Nat} (xs: Rules n (Pred α) l) (ns: Vec Bool (Symbol.nums xs)): m (Rules n (Pred α) l) := do
   return deriveLeaves xs ns
 
 class DeriveLeaveM (m: Type -> Type u) (n: Nat) (α: outParam Type) where
-  deriveLeaveM {l: Nat} (xs: Rules n (Pred α) l) (ns: List.Vector Bool (Symbol.nums xs)): m (Rules n (Pred α) l)
+  deriveLeaveM {l: Nat} (xs: Rules n (Pred α) l) (ns: Vec Bool (Symbol.nums xs)): m (Rules n (Pred α) l)
