Validator/Validator/TestMemLog.lean
@@ -1,4 +1,6 @@
 import Validator.Std.Hedge
+import Validator.Std.Vec
+
 import Validator.Parser.TokenTree
 
 import Validator.Validator.Validate
@@ -55,7 +57,7 @@ open TokenTree (node)
 #guard testCacheIsHitOnSecondRun
   (Grammar.mk (n := 1)
     (Regex.symbol (Pred.eq (Token.string "a"), 0))
-    #v[Regex.emptystr]
+    #vec[Regex.emptystr]
   )
   (node "a" []) =
   (
@@ -82,7 +84,7 @@ open TokenTree (node)
 #guard testThatTestCacheBreaksWithEmptyCache
   (Grammar.mk (n := 1)
     (Regex.symbol (Pred.eq (Token.string "a"), 0))
-    #v[Regex.emptystr]
+    #vec[Regex.emptystr]
   )
   (node "a" []) =
   Except.error "test cache miss"
@@ -90,7 +92,7 @@ open TokenTree (node)
 #guard testCacheIsHitOnSecondRun
   (Grammar.mk (n := 1)
     (Regex.symbol (Pred.eq (Token.string "a"), 0))
-    #v[Regex.emptystr]
+    #vec[Regex.emptystr]
   )
   (node "a" [node "b" []]) =
   (
@@ -125,7 +127,7 @@ open TokenTree (node)
 #guard testCacheIsHitOnSecondRun
   (Grammar.mk (n := 2)
     (Regex.symbol (Pred.eq (Token.string "a"), 0))
-    #v[
+    #vec[
       (Regex.symbol (Pred.eq (Token.string "b"), 1))
       , Regex.emptystr
     ]
@@ -163,7 +165,7 @@ open TokenTree (node)
 #guard testCacheIsHitOnSecondRun
   (Grammar.mk (n := 2)
     (Regex.symbol (Pred.eq (Token.string "a"), 0))
-    #v[
+    #vec[
       (Regex.concat
         (Regex.symbol (Pred.eq (Token.string "b"), 1))
         (Regex.symbol (Pred.eq (Token.string "c"), 1))
@@ -216,7 +218,7 @@ open TokenTree (node)
 #guard testCacheIsHitOnSecondRun
   (Grammar.mk (n := 3)
     (Regex.symbol (Pred.eq (Token.string "a"), 0))
-    #v[
+    #vec[
       (Regex.concat
         (Regex.symbol (Pred.eq (Token.string "b"), 1))
         (Regex.symbol (Pred.eq (Token.string "c"), 2))
@@ -279,7 +281,7 @@ open TokenTree (node)
 #guard testCacheIsHitOnSecondRun
   (Grammar.mk (n := 1)
     (Regex.symbol (Pred.eq (Token.string "a"), 0))
-    #v[Regex.emptystr]
+    #vec[Regex.emptystr]
   )
   (node "a" [node "b" []]) =
   (
@@ -314,7 +316,7 @@ open TokenTree (node)
 #guard testCacheIsHitOnSecondRun
   (Grammar.mk (n := 4)
     (Regex.symbol (Pred.eq (Token.string "a"), 0))
-    #v[
+    #vec[
       (Regex.concat
         (Regex.symbol (Pred.eq (Token.string "b"), 3))
         (Regex.symbol (Pred.eq (Token.string "c"), 2))
@@ -361,7 +363,7 @@ open TokenTree (node)
 #guard testCacheIsHitOnSecondRun
   (Grammar.mk (n := 2)
     (Regex.symbol (Pred.eq (Token.string "a"), 0))
-    #v[
+    #vec[
       (Regex.concat
         (Regex.symbol (Pred.eq (Token.string "b"), 1))
         Regex.emptyset
@@ -406,7 +408,7 @@ open TokenTree (node)
 #guard testCacheIsHitOnSecondRun
   (Grammar.mk (n := 3)
     (Regex.symbol (Pred.eq (Token.string "a"), 0))
-    #v[
+    #vec[
       (Regex.concat
         (Regex.symbol (Pred.eq (Token.string "b"), 1))
         (Regex.symbol (Pred.eq (Token.string "c"), 2))
@@ -468,7 +470,7 @@ open TokenTree (node)
 #guard testCacheIsHitOnSecondRun
   (Grammar.mk (n := 4)
     (Regex.symbol (Pred.eq (Token.string "a"), 0))
-    #v[
+    #vec[
       (Regex.concat
         (Regex.symbol (Pred.eq (Token.string "b"), 0))
         (Regex.symbol (Pred.eq (Token.string "c"), 1))
